\documentclass[12pt]{article}
% \documentclass[conference]{IEEEtran}

% Packages
\input{my_packages.tex}

% formatting
\input{my_format.tex}

\begin{document}
\title{Predicting Salaries From Job Descriptions}

\author{
Elijah Bernstein-Cooper, Ben Conrad, Ahmed Saif
}
\maketitle

%NB: Double ticks do not work for apostrophes, look at the output before changing all.  They do work for the first quotation mark.


    $f(\lambda)$

    \begin{equation}
        f(\lambda) = \frac{1}{6}\int_{\lambda^\prime=\lambda_0}^\lambda
                       (\lambda - \lambda^\prime)^3 f^{(4)}(\lambda^\prime){\rm
                       d}\lambda^\prime + f^{(0)}_0 + 
                       (\lambda - \lambda^\prime) f^{(1)}_0 + 
                       \frac{(\lambda - \lambda^\prime)^2}{2} f^{(2)}_0 + 
                       \frac{(\lambda - \lambda^\prime)^3}{6} f^{(3)}_0
    \end{equation}
    
    \begin{equation}
        f(\lambda) = \frac{1}{2}\int_{\lambda^\prime=\lambda_0}^\lambda
                       (\lambda - \lambda^\prime)^2 f^{(3)}(\lambda^\prime){\rm
                       d}\lambda^\prime + f^{(0)}_0 + 
                       (\lambda - \lambda^\prime) f^{(1)}_0 + 
                       \frac{(\lambda - \lambda^\prime)^2}{2} f^{(2)}_0
    \end{equation}
    
    \begin{equation}
        f(\lambda) = \int_{\lambda^\prime=\lambda_0}^\lambda
                       (\lambda - \lambda^\prime) f^{(2)}(\lambda^\prime){\rm
                       d}\lambda^\prime + f^{(0)}_0 + 
                       (\lambda - \lambda^\prime) f^{(1)}_0 
    \end{equation}
    
    \begin{equation}
        f(\lambda) = \int_{\lambda^\prime=\lambda_0}^\lambda
                       f^{(1)}(\lambda^\prime){\rm
                       d}\lambda^\prime + f^{(0)}_0
    \end{equation}

    %\begin{equation}
        \begin{align*}
            f > \epsilon_0 & \\
            {\rm d}f^2/{\rm d^2}\lambda & < 0 \\
            {\rm d}f^3/{\rm d^3}\lambda & = 0 \\
            {\rm d}f^4/{\rm d^4}\lambda & > 0
        \end{align*}
    %\end{equation}

    \begin{equation}
        R = S_1 + \chi S_2
    \end{equation}

    \begin{equation}
        S_1 = \sum^{N_{D}}_{i=1} (f_i - f^\prime_i)^2 \qquad
        S_2 = \sum^{N_{M} - 1}_{j=2} \left(\frac{{\rm d}^2 f^{\prime (4)}}{{\rm
        d}\lambda^2}\right)^2_j
    \end{equation}

    $f(\lambda)$ $N_D$ \\
    $f^\prime(\lambda^\prime)$ $N_M$ \\


    \begin{equation}
        V(\chi) = \frac{(f - f^\prime)^T (f - f^\prime) / N_D}
                       {(1 - Tr[E] / N_D)^2}
    \end{equation}

    $E$


    \begin{equation}
        \bm{f}^\prime(\lambda) = \bm{B} \bm{f}^{\prime(4)} + \bm{1}f^{(0)}_0+
        (\bm{\lambda} - \bm{1} \lambda_0) f^{\prime(1)}_0 + 
        \frac{(\bm{\lambda} - \bm{1} \lambda_0)^2}{2} f^{\prime(2)}_0 + 
        \frac{(\bm{\lambda} - \bm{1} \lambda_0)^3}{6} f^{\prime(3)}_0
    \end{equation}


    \begin{equation}
        \bm{f^{\prime (4)}_c} = (\bm{B_c}^T \bm{B_c} +
        \frac{\chi}{\Delta^4}\bm{\beta}^T
        \bm{\beta})^{-1} \bm{B_c} \bm{f}
    \end{equation}

    \begin{equation}
        \bm{f^\prime} = \bm{B}_c  \bm{f^{\prime (4)}_c}
    \end{equation}


\end{document}




